Trade/InvList: WIP on proving trade_sub_inv lemma

pulse/share/steel/examples/pulse/lib/pledge/Pulse.Lib.InvList.fst
@@ -1,6 +1,7 @@
 module Pulse.Lib.InvList
 
 open Pulse.Lib.Pervasives
+module T0 = Pulse.Lib.Priv.Trade0
 
 ```pulse
 unobservable
@@ -85,3 +86,74 @@ fn __with_invlist_ghost (#pre : vprop) (#post : vprop)
 let with_invlist_ghost = __with_invlist_ghost
 
 let invlist_reveal = admit()
+
+let iname_inj
+  (p1 p2 : vprop)
+  (i1 : inv p1) (i2 : inv p2)
+  : stt_ghost unit
+     (pure (name_of_inv i1 = name_of_inv i2))
+     (fun _ -> pure (p1 == p2))
+    = admit() // We should bubble this fact up from the memory model
+
+let invlist_mem_split (i : iname) (is : invlist)
+    (_ : squash (Set.mem i (invlist_names is)))
+    : squash (exists l r p (ii : inv p).
+              name_of_inv ii == i /\
+              is == l @ [(| p, ii |)] @ r)
+  = admit()
+
+```pulse
+ghost
+fn __invlist_sub_split
+  (is1 is2 : invlist) (_: squash (invlist_sub is1 is2))
+  requires invlist_v is2
+  ensures  invlist_v is1 ** T0.stick (invlist_v is1) (invlist_v is2)
+{
+  open T0;
+  match is1 {
+    Nil -> {
+      ghost fn aux (_:unit)
+        requires invlist_v is2 ** invlist_v is1
+        ensures invlist_v is2
+      {
+        rewrite invlist_v is1 as emp;
+        ();
+      };
+      intro_stick (invlist_v is1) (invlist_v is2) (invlist_v is2) aux;
+      rewrite emp as invlist_v is1;
+    }
+    Cons h t -> {
+      let p = dfst h;
+      let i : inv p = dsnd h;
+      let name = name_of_inv i;
+      (* This is the interesting case, but it's rather hard to prove right now
+      due to some pulse limitations (#151, #163). The idea is that (p, i) must
+      also be in is2, so we can rewrite
+           invlist_v is2
+        ~> invlist_v (l @ [(|p, i|)] @ r)
+        ~> p ** invlist_v (l @ r)
+
+      and prove invlist_sub t (l@r), then we call the lemma recursively to obtain
+          p ** invlist_v t ** stick (invlist_v t) (invlist_v (l@r))
+        ~> invlist_v is1 ** stick (invlist_v t) (invlist_v (l@r))
+      then we can 'frame' the stick with 'p' to get
+        ~> invlist_v is1 ** stick (p ** invlist_v t) (p ** invlist_v (l@r))
+        ~> invlist_v is1 ** stick is1 is2
+      *)
+      admit();
+    }
+  }
+}
+```
+
+```pulse
+ghost
+fn __invlist_sub_split_wrap
+  (is1 is2 : invlist)
+  requires pure (invlist_sub is1 is2) ** invlist_v is2
+  ensures  invlist_v is1 ** Pulse.Lib.Priv.Trade0.stick (invlist_v is1) (invlist_v is2)
+{
+  __invlist_sub_split is1 is2 ()
+}
+```
+let invlist_sub_split = __invlist_sub_split_wrap
